theories/FOL/Reductions/H10p_to_FA.v
@@ -14,8 +14,8 @@ Fixpoint embed_poly p : term :=
 
   
 (* We translate h10 problems to formulas in PA *)
-Definition embed_problem (E : H10p_PROBLEM) : form := let (a, b) := E in
-                                                      embed_poly a == embed_poly b.
+Definition embed_problem (E : H10p_PROBLEM) : form :=
+  let (a, b) := E in embed_poly a == embed_poly b.
 
 Definition H10p_sem E sigma := dp_eval_pfree sigma (fst E) = dp_eval_pfree sigma (snd E).
 
@@ -33,8 +33,9 @@ Proof.
   - reflexivity.
   - cbn. rewrite iter_switch.
     change (iter _ _ _) with (exist_times N (∃ phi)).
-    setoid_rewrite IHN.
-Admitted.
+    setoid_rewrite IHN. symmetry.
+    now apply bounded_S_exists.
+Qed.
 
 
 Lemma embed_is_closed E : bounded 0 (embed E).
@@ -46,7 +47,7 @@ Qed.
 
 
 Lemma prv_poly sigma q Gamma :
-  incl FA_facts.FA Gamma -> Gamma ⊢I ( (embed_poly q)`[sigma >> num] == num (dp_eval_pfree sigma q) ).
+  incl FAeq Gamma -> Gamma ⊢I ( (embed_poly q)`[sigma >> num] == num (dp_eval_pfree sigma q) ).
 Proof.
   intros H.
   induction q; cbn.
@@ -55,7 +56,7 @@ Proof.
     now apply reflexivity.
   - now apply reflexivity.
   - destruct d; cbn.
-    + eapply transitivity. assumption. 
+    + eapply transitivity. assumption.
       apply (eq_add _ _ H IHq1 IHq2).
       now apply num_add_homomorphism.
     + eapply transitivity. assumption.
@@ -66,9 +67,9 @@ Qed.
 
 
 Lemma problem_to_prv :
-  forall E sigma, H10p_sem E sigma -> FA_facts.FA ⊢I (embed_problem E)[sigma >> num].
+  forall E sigma, H10p_sem E sigma -> FAeq ⊢I (embed_problem E)[sigma >> num].
 Proof.
-  intros [a b] sigma HE. cbn -[FA].
+  intros [a b] sigma HE. cbn -[FAeq].
   eapply transitivity; firstorder.
   apply prv_poly; firstorder.
   apply symmetry; firstorder.
@@ -78,43 +79,58 @@ Qed.
 
 
 
-  Section FA_Model.
+Section FA_Model.
 
-    Context {D : Type}.
-    Context {I : interp D}.
+  Context {D : Type}.
+  Context {I : interp D}.
 
-    Hypothesis ext_model : extensional I.
-    Hypothesis FA_model : forall rho ax, In ax FA_facts.FA -> rho ⊨ ax.
+  Hypothesis ext_model : extensional I.
+  Hypothesis FA_model : forall rho ax, In ax FAeq -> rho ⊨ ax.
 
-    
-    Fact eval_num sigma n : eval sigma (num n) = iμ n.
-    Proof.
-      induction n.
-      - reflexivity.
-      - cbn. now rewrite IHn.
-    Qed.
+  Notation "'iO'" := (i_func (f:=Zero) (Vector.nil D)) (at level 2) : PA_Notation.  
 
-    Notation "'iO'" := (i_func (f:=Zero) (Vector.nil D)) (at level 2) : PA_Notation.
-    
-    Lemma problem_to_model E sigma : H10p_sem E sigma -> (sigma >> iμ) ⊨ embed_problem E.
-    Proof.
-      intros HE%problem_to_prv%soundness.
-      specialize (HE D I).
-      setoid_rewrite sat_comp in HE.
-      eapply sat_ext. 2: apply HE.
-      intros x. unfold ">>". now rewrite eval_num.
-      intros. instantiate (1 := (fun _ => iO)).
-      now apply FA_model.  
-    Qed.
-    
-    
-  End FA_Model.
+  Lemma problem_to_model E sigma : H10p_sem E sigma -> (sigma >> iμ) ⊨ embed_problem E.
+  Proof.
+    intros HE%problem_to_prv%soundness.
+    specialize (HE D I).
+    setoid_rewrite sat_comp in HE.
+    eapply sat_ext. 2: apply HE.
+    intros x. unfold ">>". now rewrite eval_num.
+    intros. instantiate (1 := (fun _ => iO)).
+    now apply FA_model.
+  Qed.
+   
+End FA_Model.
 
 
+Fact nat_eval_poly (sigma : env nat) p :
+  @eval _ _ _ interp_nat sigma (embed_poly p) = dp_eval_pfree sigma p.
+Proof.
+  induction p; cbn.
+  - now rewrite nat_eval_num.
+  - reflexivity.
+  - destruct d; cbn.
+    + now rewrite IHp1, IHp2.
+    + now rewrite IHp1, IHp2.
+Qed.
+
+Lemma nat_sat :
+  forall E rho, sat interp_nat rho (embed_problem E) <-> H10p_sem E rho.
+Proof.
+  intros E rho. split.
+  - destruct E as [a b]. unfold H10p_sem. cbn.
+    now rewrite !nat_eval_poly.
+  - intros. eapply (@sat_ext _ _ _ _ _ (rho >> @iμ nat interp_nat)).
+    intros x. change ((rho >> iμ) x) with (@iμ nat interp_nat (rho x)).
+    induction (rho x). reflexivity. cbn. now rewrite IHn.
+    eapply problem_to_model.
+    apply nat_is_FA_model.
+    assumption.
+Qed.
 
 
 Theorem Reduction_sat :
-  forall E, H10p_SAT E <-> valid_ctx FA_facts.FA (embed E).
+  forall E, H10p_SAT E <-> valid_ctx FAeq (embed E).
 Proof.
   split.
   - intros [sigma HE].
@@ -123,20 +139,20 @@ Proof.
     apply problem_to_model.
     + intros ρ' ax Hax. eapply sat_closed.
       2: now apply H.
-    (* repeat (destruct Hax as [<- | Hax]; auto). *)
+      (* repeat (destruct Hax as [<- | Hax]; auto). *)
       admit.
     + apply HE.
     + rewrite <-exists_close_form; apply embed_is_closed.
   - intros H.
-    (* specialize (H nat interp_nat id (nat_is_FA_model id)). *)
-    (* unfold embed in *. apply subst_exist_sat2 in H. *)
-    (* destruct H as [sigma Hs]. exists sigma. *)
-    (* now apply nat_sat. *)
+    specialize (H nat interp_nat id (nat_is_FA_model id)).
+    unfold embed in *. apply subst_exist_sat2 in H.
+    destruct H as [sigma Hs]. exists sigma.
+    now apply nat_sat.
 Admitted.
 
 
 
-Theorem Reduction_prv : forall E, H10p_SAT E <-> FA_facts.FA ⊢I embed E.
+Theorem Reduction_prv : forall E, H10p_SAT E <-> FAeq ⊢I embed E.
 Proof.
   intros E. split.
   - intros [sigma HE].
@@ -144,8 +160,8 @@ Proof.
     apply problem_to_prv,  HE.
     rewrite <-exists_close_form; apply embed_is_closed.
   - intros H%soundness.
-    (* now apply Reduction_sat. *)
-Admitted.
+    now apply Reduction_sat.
+Qed.
 
 
 
