theories/FOL/PA_undec.v
@@ -1,43 +1,42 @@
 Require Import Undecidability.Synthetic.Definitions Undecidability.Synthetic.Undecidability.
 Require Import Undecidability.FOL.PA.
-Require Import List.
-From Undecidability.FOL.Util Require Import FullTarski FullDeduction_facts.
+From Undecidability.FOL.Util Require Import FullTarski.
 From Undecidability.H10 Require Import H10p H10p_undec.
+From Undecidability.FOL.Reductions Require Import H10p_to_FA.
 
 
-Definition standard {I} (M : interp I) := True.
 
-Theorem H10_entailment_FA :
-  (exists I (M : interp I), extensional M /\ standard M /\ forall rho psi, In psi FA -> rho ⊨ psi) -> H10p_SAT ⪯ entailment_FA.
+Theorem H10_entailment_FA : H10p_SAT ⪯ entailment_FA.
 Proof.
-Admitted.
+  exists embed. intros E. apply Reduction_sat.
+Qed.
 
 
-Theorem H10_entailment_PA :
-  (exists I (M : interp I), extensional M /\ standard M /\ forall rho psi, PA psi -> rho ⊨ psi) -> H10p_SAT ⪯ entailment_PA.
+Corollary H10_entailment_PA : H10p_SAT ⪯ entailment_PA.
 Proof.
+  exists embed. intros E; split.
+  - 
 Admitted.
 
 
 Theorem H10_deduction_FA : H10p_SAT ⪯ deduction_FA.
 Proof.
-Admitted.
+  exists embed. intros E. apply Reduction_prv.
+Qed.
 
 
-Theorem H10_deduction_PA : H10p_SAT ⪯ deduction_PA.
+Corollary H10_deduction_PA : H10p_SAT ⪯ deduction_PA.
 Proof.
 Admitted.
-
 
 
 
 Theorem undecidable_entailment_PA :
-  (exists I (M : interp I), extensional M /\ standard M /\ forall rho psi, PA psi -> rho ⊨ psi) -> undecidable entailment_PA.
+  undecidable entailment_PA.
 Proof.
-  intros H. refine (undecidability_from_reducibility _ (H10_entailment_PA H)).
+  refine (undecidability_from_reducibility _ H10_entailment_PA).
   apply H10p_undec.
 Qed.
-
 
 
 Theorem undecidable_deduction_PA : undecidable deduction_PA.
